ExtraLists.v
@@ -1,0 +1,102 @@
+Require Import NArith.
+Require Import UROP.Types.
+Require Import Lia.
+
+Local Open Scope UROP_scope.
+
+Ltac simplify_list :=
+  try match goal with
+  | [|- context[Datatypes.length (List.map _ _)]] => rewrite List.map_length
+  | [|- context[Datatypes.length (List.repeat _ _)]] => rewrite List.repeat_length
+  | [|- context[List.firstn 0 _]] => rewrite List.firstn_O
+  | [|- context[_ ++l []]] => rewrite List.app_nil_r
+  | [|- context[List.length (List.firstn _ _)]] => rewrite List.firstn_length
+  | [|- context[Datatypes.length (_ ++l _)]] => rewrite List.app_length
+  | [H: (_ < 0)%nat |- _] => inversion H
+  | [|- context[List.firstn (S _) (_ :: _)]] => rewrite List.firstn_cons
+  | [|- context[List.skipn (S _) (_ :: _)]] => rewrite List.skipn_cons
+  | [|- context[List.nth _ (List.repeat _ _) _]] => rewrite List.nth_repeat
+  (*| [|- context[List.firstn _ (_ ++l _)]] => rewrite List.firstn_app*)
+  | _ => idtac
+  end; simpl; eauto.
+
+Ltac lists := repeat simplify_list.
+
+(* List Helper Lemmas {{{ *)
+Lemma list_fact {A} : forall n m (l : list A) d,
+  lt n m
+  -> ge (List.length l) m
+  -> List.nth n (List.firstn m l) d = List.nth n l d.
+Proof.
+  intros.
+  replace (List.nth n l d) with (List.nth n (List.firstn m l ++l List.skipn m l) d).
+  Search (List.nth).
+  rewrite List.app_nth1; eauto.
+  rewrite List.firstn_length; lia.
+  rewrite List.firstn_skipn; eauto.
+Qed.
+
+Lemma rev_rev {A} : forall (l : list A),
+  List.NoDup (List.rev l) -> List.NoDup l.
+Proof.
+  intros.
+  apply List.NoDup_rev in H.
+  rewrite List.rev_involutive in H.
+  assumption.
+Qed.
+
+Open Scope list_scope.
+Lemma zip_app {A} {B} : forall (a1 : list A) (b1 : list B) a2 b2,
+  List.length a1 = List.length b1
+  -> zip (a1 ++ a2) (b1 ++ b2) = zip a1 b1 ++ zip a2 b2.
+Proof.
+  induction a1; induction b1; eauto.
+  inversion 1.
+  inversion 1.
+  intros; simpl.
+  f_equal.
+  eauto.
+Qed.
+
+Lemma zip_length {A} {B} : forall (a : list A) (b : list B),
+  List.length (zip a b) = Nat.min (List.length a) (List.length b).
+Proof.
+  induction a; induction b; simpl; eauto.
+Qed.
+Close Scope list_scope.
+
+Lemma list_firstn_skipn_succ : forall A (l : list A) i d,
+  lt i (List.length l) ->
+  List.skipn i (List.firstn (i+1) l) = [List.nth i l d].
+Proof.
+  induction l.
+  inversion 1.
+
+  lists.
+  intros.
+  destruct i.
+  lists.
+  replace ((S i + 1)%nat) with (S (i + 1)) by lia.
+  lists.
+  apply IHl.
+  lia.
+Qed.
+
+Lemma list_firstn_succ : forall A (l : list A) i d,
+  lt i (List.length l) ->
+  List.firstn (S i) l = (List.firstn i l ++l [List.nth i l d]).
+Proof.
+  induction l.
+  inversion 1.
+
+  lists.
+  intros.
+  destruct i.
+  lists.
+  replace ((S i + 1)%nat) with (S (i + 1)) by lia.
+  lists.
+  f_equal.
+  apply IHl.
+  lia.
+Qed.
+(* }}} *)
