Tactics.v
@@ -1,5 +1,6 @@
 Require Import NArith.
 Require Import UROP.Types.
+Require Import UROP.ExtraLists.
 (*Require Import UROP.BitVectors.*)
 
 Local Open Scope UROP_scope.
@@ -15,23 +16,7 @@ Ltac propositional :=
   | [H: _ /\ _ |- _] => inversion H; clear H
   end.
 
-Ltac simplify_list :=
-  try match goal with
-  | [|- context[Datatypes.length (List.map _ _)]] => rewrite List.map_length
-  | [|- context[Datatypes.length (List.repeat _ _)]] => rewrite List.repeat_length
-  | [|- context[List.firstn 0 _]] => rewrite List.firstn_O
-  | [|- context[_ ++l []]] => rewrite List.app_nil_r
-  | [|- context[List.length (List.firstn _ _)]] => rewrite List.firstn_length
-  | [|- context[Datatypes.length (_ ++l _)]] => rewrite List.app_length
-  | [H: (_ < 0)%nat |- _] => inversion H
-  | [|- context[List.firstn (S _) (_ :: _)]] => rewrite List.firstn_cons
-  | [|- context[List.skipn (S _) (_ :: _)]] => rewrite List.skipn_cons
-  | [|- context[List.nth _ (List.repeat _ _) _]] => rewrite List.nth_repeat
-  (*| [|- context[List.firstn 0 _]] => rewrite List.firstn_O*)
-  | _ => idtac
-  end; simpl; eauto.
-
-Ltac lists := repeat simplify_list.
+Ltac simplify := autorewrite with core; simpl.
 
 (*Local Hint Rewrite N_to_bvM_length : core.
    Local Hint Rewrite var_names_length : core.*)
